

Note on Average Null Energy Condition

Ruihua Fan

Department of Physics, Harvard University, Cambridge, MA 02138, USA

Abstract

Note on average null energy condition. Use (1+1)D free boson as an example to show, how it is satisfied in general and when it will be violated.

Contents

1	Perturb the vacuum	2
2	Change the Hamiltonian	3
A	Details for the calculation	3

Einstein gravity theory tells us the metric is determined by the matters. However, it doesn't tell us anything about the matter. Energy conditions are some constraints on the matters [1]. Average null energy condition is one of them and stated in the following form,

$$\int dx^+ T_{++} \geq 0, \quad \int dx^- T_{--} \geq 0. \quad (1)$$

It is also related to causality. Here we're not going to talk about this AVEG generally. Instead, the purpose of this note is very modest: we are going to use free boson as an example to show how it is satisfied and how to break it.

We choose the following action [3],

$$S = \frac{g}{2} \int d^2x (\partial_t \varphi)^2 - (\partial_x \varphi)^2, \quad (2)$$

which boundary condition $\varphi(x) = \varphi(x + L)$. Under canonical quantization, the field operator can be expanded as,

$$\varphi(x, t) = \varphi_0 + \frac{1}{gL} \pi_0 t + \frac{i}{\sqrt{4\pi g}} \sum_{n \neq 0} \frac{1}{n} (a_n e^{2\pi i n(x-t)/L} - \bar{a}_{-n} e^{2\pi i n(x+t)/L}) \quad (3)$$

φ_0 and π_0 describe the center of mass motion. a_n, \bar{a}_n are the left and right movers moving along the lightcone direction with finite momentum, which satisfy a set of commutators,

$$[a_n, a_m] = n\delta_{n+m}, \quad [\bar{a}_n, \bar{a}_m] = n\delta_{n+m}, \quad [a_n, \bar{a}_m] = 0. \quad (4)$$

And in the following discussion, for simplicity, we will use lightcone coordinate,

$$x^+ = x + t, \quad x^- = x - t, \quad (5)$$

where the energy-momentum tensor has a simpler form,

$$T_{--} = g\partial_- \varphi \partial_- \varphi, \quad T_{++} = g\partial_+ \varphi \partial_+ \varphi, \quad T_{-+} = 0. \quad (6)$$

1 Perturb the vacuum

First, we want to use a non-local unitary to perturb the vacuum state, then measure the energy-momentum tensor, i.e.

$$\langle T_{--} \rangle_p = \langle 0 | e^{-i\lambda \varphi_L \varphi_R} T_{--}(x) e^{i\lambda \varphi_L \varphi_R} | 0 \rangle = -i\lambda \langle 0 | [\varphi_L \varphi_R, T_{--}(x)] | 0 \rangle. \quad (7)$$

where $\varphi_L = \varphi(-x_0, 0)$, $\varphi_R = \varphi(x_0, 0)$, which can be thought of as two sources of left and right movers. In the last step, we do a expansion w.r.t. λ and use $\langle T_{--}(x) \rangle = 0$. So up to this order, we have

$$\langle T_{--} \rangle_p = -i\lambda \left(\langle 0 | [\varphi_L, \partial_- \varphi] \varphi_R \partial_- \varphi | 0 \rangle + \langle 0 | \partial_- \varphi [\varphi_L, \partial_- \varphi] \varphi_R | 0 \rangle + \right. \quad (8)$$

$$\left. \langle 0 | \varphi_L [\varphi_R, \partial_- \varphi] \partial_- \varphi | 0 \rangle + \langle 0 | \varphi_L \partial_- \varphi [\varphi_R, \partial_- \varphi] | 0 \rangle \right). \quad (9)$$

Using the mode expansion formula, one can show that (See Appendix.A),

$$[\varphi(x_1, t_1), \partial_- \varphi(x_2, t_2)] = -\frac{i}{2g} \delta(x_1^- - x_2^-), \quad (10)$$

$$\langle \varphi(x_1, t_1) \partial_- \varphi(x_2, t_2) \rangle + \langle \partial_- \varphi(x_2, t_2), \varphi(x_1, t_1) \rangle = \frac{1}{2\pi g} P \frac{1}{x_1^- - x_2^-}. \quad (11)$$

So that we have

$$\langle T_{--}(x) \rangle_p = \frac{-\lambda}{4\pi g^2} \frac{\delta(x_L^- - x^-)}{x_R^- - x_L^-} - \frac{-\lambda}{4\pi g^2} \frac{\delta(x_R^- - x^-)}{x_L^- - x_R^-}. \quad (12)$$

Because $x_R^- x_L^- = 2x_0 > 0$, the two terms have opposite signs thus cancel each other, which preserves the ANEC.

2 Change the Hamiltonian

Another scenario is to change the Hamiltonian by adding a time-dependent non-local term, which breaks Lorentz symmetry and locality,

$$H = H_0 + \delta(t)\lambda\varphi_L\varphi_R. \quad (13)$$

where φ_L and φ_R follow the same definition above. The Heisenburg operators evolving under this new Hamiltonian is written as $\tilde{O}(x)$. Now we have,

$$t < 0, \quad \langle \tilde{T}_{--}(x) \rangle = \langle T_{--}(x) \rangle = 0; \quad (14)$$

$$t > 0, \quad \langle \tilde{T}_{--}(x) \rangle = \langle 0 | e^{-i\lambda\varphi_L\varphi_R} T_{--}(x) e^{i\lambda\varphi_L\varphi_R} | 0 \rangle. \quad (15)$$

So this time, ANEC is violated for x^- slides between $-x_0$ and x_0 .

From this calculation, it seems that the coupling term $\varphi_L\varphi_R$ is not essential. If we only add φ_L or φ_R , the AVNE can also be violated.

A Details for the calculation

We first consider the commutator between two boson fields,

$$\begin{aligned} [\varphi(x_1, t_1), \varphi(x_2, t_2)] &= \frac{1}{gL} \left([\pi_0 t_1, \varphi_0] + [\varphi_0, \pi_0 t_2] \right) \\ &\quad + \frac{-1}{4\pi g} \left[\sum_{n \neq 0} \frac{1}{n} a_n e^{2\pi i n x_1^- / L}, \sum_{m \neq 0} \frac{1}{m} a_m e^{2\pi i m x_2^- / L} \right] \\ &\quad + \frac{-1}{4\pi g} \left[\sum_{n \neq 0} \frac{1}{n} \bar{a}_{-n} e^{2\pi i n x_1^+ / L}, \sum_{m \neq 0} \frac{1}{m} \bar{a}_{-m} e^{2\pi i m x_2^+ / L} \right] \\ &= \frac{-i}{gL} (t_1 - t_2) + \frac{1}{4\pi g} \sum_{n \neq 0} \frac{1}{n} \left(e^{2\pi i n (x_1^- - x_2^-) / L} + e^{2\pi i n (x_1^+ - x_2^+) / L} \right). \end{aligned}$$

Using this, we have,

$$\begin{aligned} [\varphi(x_1, t_1), \partial_- \varphi(x_2, t_2)] &= \frac{-i}{2gL} \sum_{n=-\infty}^{\infty} e^{2\pi i n (x_1^- - x_2^-) / L} \\ &= \frac{-i}{2g} \sum_{k=-\infty}^{\infty} \delta((x_1^- - x_2^-) - kL) \end{aligned} \quad (16)$$

$$\xrightarrow{L \rightarrow \infty} \frac{-i}{2g} \delta(x_1^- - x_2^-). \quad (17)$$

From the first to the second line, we use Poisson summation formula $\frac{1}{T} \sum_{k=-\infty}^{\infty} e^{2\pi i k x / T} = \sum_{n=-\infty}^{\infty} \delta(x - nT)$.

Then let's compute the correlation functions,

$$\begin{aligned}
\langle \varphi(x_1, t_1) \partial_- \varphi(x_2, t_2) \rangle &= \langle 0 | \left(\varphi_0 + \frac{1}{gL} \pi_0 t_1 \right) \frac{-\pi_0}{2gL} | 0 \rangle \\
&\quad + \langle 0 | \frac{i}{\sqrt{4\pi g}} \sum_{n \neq 0} \frac{1}{n} a_n e^{2\pi i n x_1^- / L} \frac{i}{\sqrt{4\pi g}} \sum_{m \neq 0} \frac{1}{m} \frac{2\pi i m}{L} a_m e^{2\pi i m x_2^- / L} | 0 \rangle \\
&= \langle 0 | \left(\varphi_0 + \frac{1}{gL} \pi_0 t_1 \right) \frac{-\pi_0}{2gL} | 0 \rangle - \frac{i}{2gL} \sum_{n > 0} e^{2\pi i n (x_1^- - x_2^-) / L}. \\
\langle \partial_- \varphi(x_2, t_2) \varphi(x_1, t_1) \rangle &= \langle 0 | \frac{-\pi_0}{2gL} \left(\varphi_0 + \frac{1}{gL} \pi_0 t_1 \right) | 0 \rangle + \frac{i}{2gL} \sum_{n > 0} e^{2\pi i n (x_2^- - x_1^-) / L}.
\end{aligned}$$

In the thermodynamic limit, we can drop the contribution from zero mode. For the $n > 0$ modes, we use the formula

$$\frac{1}{L} \sum_{n=1}^{\infty} e^{2\pi i n x / L} = \int_0^{\infty} \frac{dk}{2\pi} e^{ikx} = \int_0^{\infty} \frac{dk}{2\pi} e^{ik(x+i\epsilon)} = \frac{1}{2\pi} \frac{i}{x+i\epsilon} = \frac{i}{2\pi} \left(P \frac{1}{x} - i\pi \delta(x) \right),$$

which leads to,

$$\langle \varphi(x_1, t_1) \partial_- \varphi(x_2, t_2) \rangle + \langle \partial_- \varphi(x_2, t_2) \varphi(x_1, t_1) \rangle = \frac{1}{2\pi g} P \frac{1}{x_1^- - x_2^-}. \quad (18)$$

All of these calculations can be easily extended to T_{++} .

References

- [1] A. Zee, “Einstein gravity in a nutshell”, *Princeton*.
- [2] D. Stanford, “talk at the conference celebrating Hawking’s birthday”.
- [3] F. D. Francesco, *et.al.*, “Conformal Field theory”, *Springer*.